\begin{proof}
  By induction on the structure of programs.
  \begin{case}
  \item$p=\ceu\Term$.  Then there is no such $\delta$ (no rule applicable).
    And by~\Cref{def:orig:blocked},
    $\blocked(\ceu\Term,\alpha,n)=1$.
    %%
  \item$p=\ceu\Fin$.  Then there is no such $\delta$ (no rule applicable).
    And by~\Cref{def:orig:blocked},
    $\blocked(\ceu\Fin,\alpha,n)=1$.
    %%
  \item$p=\ceu\Skip$.  Then by axiom~\eqref{def:orig:inner:skip},
    \[
      \<\ceu\Skip,\alpha,m>
      \step{n}\<\ceu\Term,\alpha,m>=\delta.
    \]
    And by~\Cref{def:orig:blocked}, $\blocked(\ceu\Skip,\alpha,n)=0$.
    %%
  \item$p=\ceu{\Attr{v}{a}}$.  Then by axiom~\eqref{def:orig:inner:attr},
    \[
      \<\ceu{\Attr{v}{a}},\alpha,m>
      \step{n}\<\ceu\Skip,\alpha,m[v/\eval(a)]>=\delta.
    \]
    And by~\Cref{def:orig:blocked}, $\blocked(\ceu{\Attr{v}{a}},\alpha,n)=0$.
    %%
  \item $p=\ceu{\Await(e)}$.  Then by axiom~\eqref{def:orig:inner:await},
    \[
      \<\ceu{\Await(e)},\alpha,m>
        \step{n}\<\ceu{\Awaiting(e,n')},\alpha,m>=\delta,
    \]
    where $n'=n+1$.  And by~\Cref{def:orig:blocked},
    $\blocked(\ceu{\Await(e)},\alpha,n)=0$.
    %%
  \item $p=\ceu{\Awaiting(e,n')}$.
    \begin{case}
    \item$n'\leq n$.  If~$e$ is the top-of-stack event in~$\alpha$, in
      symbols~$e=\alpha_{[1]}$, then by
      axiom~\eqref{def:orig:inner:awaiting},
      \[
        \<\ceu{\Awaiting(e,n')},\alpha,m>
        \step{n}\<\ceu{\Skip},\alpha,m>=\delta,
      \]
      and by \Cref{def:orig:blocked},
      $\blocked(\ceu{\Awaiting(e,n')},\alpha,n)=0$.

      If, however, $e\ne\alpha_{[1]}$, then there is no such~$\delta$, as no
      rule is applicable.  And by \Cref{def:orig:blocked},
      $\blocked(\ceu{\Awaiting(e,n')},\alpha,n)=1.$
    %%
    \item$n'>n$. Then there is no such~$\delta$ (no rule applicable).
      And by~\Cref{def:orig:blocked},
      $\blocked(\ceu{\Awaiting(e,n')},\alpha,n)=1$.
    \end{case}
    %%
  \item$p=\ceu{\Emit(e)}$.  Then by axiom~\eqref{def:orig:inner:emit},
    \[
      \<\ceu{\Emit(e)},\alpha,m>
      \step{n}\<\ceu{\Emitting(n')},e\alpha,m>=\delta,
    \]
    where~$n'=\|\alpha|$.  And by~\Cref{def:orig:blocked},
    $\blocked(\ceu{\Emit(e')},e\alpha,n)=0$.
    %%
  \item $p=\ceu{\Emitting(e,n')}$.
    \begin{case}
    \item~$n'=\|\alpha|$.  By axiom~\eqref{def:orig:inner:emitting},
      \[
        \<\ceu{\Emitting(e,n')},\alpha,m>
        \step{n}\<\ceu{\Skip},\alpha,m>=\delta.
      \]
      And by \Cref{def:orig:blocked},
      $\blocked(\ceu{\Emitting(e,n')},\alpha,n)=0$.
    %%
    \item~$n'\ne\|\alpha|$.  Then there is no such~$\delta$ (no rule is
      applicable) and, by \Cref{def:orig:blocked},
      $\blocked(\ceu{\Emitting(e,n')},\alpha,n)=1$.
    \end{case}
    %%
  \item $p=\ceu{\Ifelse{b}{p'}{p''}}$.  By
    axioms~\eqref{def:orig:inner:if-true}
    and~\eqref{def:orig:inner:if-false}, if~$\eval(b,m)=1$,
    $\delta=\<p',\alpha,m>$, otherwise~$\delta=\<p'',\alpha,m>$.  And
    by~\Cref{def:orig:blocked},
    \[
      \blocked(\ceu{\Ifelse{b}{p'}{p''}},e\alpha,n)=0.
    \]
    %%
  \item$p=\ceu{p';p''}$.
    \begin{case}
    \item$p'=\ceu{\Skip}$.  By axiom~\eqref{def:orig:inner:seq-skip},
      $\delta=\<p'',\alpha,m>$, and by~\Cref{def:orig:blocked},
      \[
        \blocked(\ceu{\Skip};p'', \alpha,n)
        =\blocked(\ceu{\Skip},\alpha,n)=0.
      \]
    \item$p'=\ceu\Break$.  By axiom~\eqref{def:orig:inner:seq-break},
      $\delta=\<\ceu\Break,\alpha,m>$, and by~\Cref{def:orig:blocked},
      \[
        \blocked(\ceu{\Break};p'',\alpha,n)
        =\blocked(\ceu{\Break},\alpha,n)=0.
      \]
    \item$p'\ne\ceu{\Skip},\ceu{\Break}$.  By induction
      hypothesis, exactly one of the following hold:
      \[
        \exists{d'\in\Delta}(\<p',\alpha,m>\step{n}d')
        \quad\text{or}\quad
        \blocked(p',\alpha,n)=1.
      \]

      If~$\<p',\alpha,m>\step{n}\<p_1',\alpha',m'>$, for some~$p_1'\in{P}$,
      $\alpha'\in{E^*}$, and~$m'\in\mathcal{M}$, then by
      rule~\eqref{def:orig:inner:seq},
      \[
        \<p';p'',\alpha,m>\step{n}\<p'_1;p'',\alpha',m'>,
      \]
      and by \Cref{def:orig:blocked},
      \[
        \blocked(p';p'',\alpha,n)=\blocked(p',\alpha,n)=0.
      \]

      If, however, $\blocked(p',\alpha,n)=1$, then there is no such~$d$ (no
      rule is applicable) and by \Cref{def:orig:blocked},
      \[
        \blocked(p';p'',\alpha,n)=\blocked(p',\alpha,n)=1.
      \]
    \end{case}
    %%
  \item$p=\ceu{\Loop{p'}}$.  By axiom~\eqref{def:orig:inner:loop},
    $\delta=\<\ceu{p'\Atloop{p'}},\alpha,m>$.  And
    by~\Cref{def:orig:blocked}, $\blocked(\ceu{\Loop{p'}},\alpha,m)=0$.
    %%
  \item$p=\ceu{p'\Atloop{p''}}$.
    \begin{case}
    \item$p'=\ceu{\Skip}$.  By axiom~\eqref{def:orig:inner:atloop-skip},
      $\delta=\<\ceu{\Loop{p''}},\alpha,m>$, and by~\Cref{def:orig:blocked},
      \[
        \blocked(\ceu{\Skip\Atloop{p''}},\alpha,n)
        =\blocked(\ceu{\Skip},\alpha,n)=0.
      \]
    \item$p'=\ceu{\Break}$.  By axiom~\eqref{def:orig:inner:atloop-break},
      $\delta=\<\ceu{\Skip},\alpha,m>$, and by~\Cref{def:orig:blocked},
      \[
        \blocked(\ceu{\Break\Atloop{p''}},\alpha,n)
        =\blocked(\ceu{\Break},\alpha,n)=0.
      \]
    \item$p'\ne\ceu{\Skip},\ceu{\Break}$.  By induction
      hypothesis, exactly one of the following hold:
      \[
        \exists{d'\in\Delta}(\<p',\alpha,m>\step{n}d')
        \quad\text{or}\quad
        \blocked(p',\alpha,n)=1.
      \]

      If~$\<p',\alpha,m>\step{n}\<p_1',\alpha',m'>$, for some~$p_1'\in{P}$,
      $\alpha'\in{E^*}$, and~$m'\in\mathcal{M}$, then by
      rule~\eqref{def:orig:inner:atloop},
      \[
        \<\ceu{p'\Atloop{p''}},\alpha,m>
        \step{n}\<\ceu{p'_1\Atloop{p''}},\alpha',m'>,
      \]
      and by \Cref{def:orig:blocked},
      \[
        \blocked(\ceu{p'\Atloop{p''}},\alpha,n)=\blocked(p',\alpha,n)=0.
      \]

      If, however,~$\blocked(p',\alpha,n)=1$, then there is no such~$d$ (no
      rule is applicable) and by \Cref{def:orig:blocked},
      \[
        \blocked(\ceu{p'\Atloop{p''}},\alpha,n)=\blocked(p',\alpha,n)=1.
      \]
    \end{case}
    %%
  \item$p=\ceu{p'\And{p''}}$.
    \begin{case}
    \item$p'=\ceu{\Skip}$.  By axiom~\eqref{def:orig:inner:and-skip-left},
      $\delta=\<\ceu{p''},\alpha,m>$, and by~\Cref{def:orig:blocked},
      \begin{align*}
        \blocked(\ceu{\Skip\And\;p''},\alpha,n)
        &=\blocked(\ceu{\Skip},\alpha,n)
          \cdot\blocked(p'',\alpha,n)\\
        &=0.
      \end{align*}
    \item $p'\ne\ceu{\Skip,\Break}$ and~$p''=\ceu{\Skip}$.  By
      induction hypothesis, exactly one of the following hold:
      \[
        \exists{d'\in\Delta}(\<p',\alpha,m>\step{n}d')
        \quad\text{or}\quad
        \blocked(p',\alpha,n)=1.
      \]

      If~$\blocked(p',\alpha,n)=0$, this case
      becomes~\Cref{thm:orig:lemma:and}.

      If, however,~$\blocked(p',\alpha,n)=1$, then by
      axiom~\eqref{def:orig:inner:and-skip-right},
      $\delta=\<\ceu{p'},\alpha,m>$, and by \Cref{def:orig:blocked},
      \begin{align*}
        \blocked(\ceu{p'\And\;\Skip},\alpha,n)
        &=\blocked(p',\alpha,n)\cdot\blocked(\ceu\Skip,\alpha,n)\\
        &=1\cdot0=0.
      \end{align*}
    \item$p'=\ceu{\Break}$.  By axiom~\eqref{def:orig:inner:and-break-left},
      $\delta=\<\ceu{\clear(p'')},\alpha,m>$, and
      by~\Cref{def:orig:blocked},
      \begin{align*}
        \blocked(\ceu{\Break\And\;p''})
        &=\blocked(\ceu{\Break},\alpha,n)\cdot\blocked(p'',\alpha,n)\\
        &=0.
      \end{align*}
    \item $p'\ne\ceu{\Skip,\Break}$ and~$p''=\ceu\Break$.  By
      induction hypothesis, exactly one of the following hold:
      \[
        \exists{d'\in\Delta}(\<p',\alpha,m>\step{n}d')
        \quad\text{or}\quad
        \blocked(p',\alpha,n)=1.
      \]

      If~$\blocked(p',\alpha,n)=0$, this case becomes
      \Cref{thm:orig:lemma:and}.

      If, however,~$\blocked(p',\alpha,n)=1$, then by
      axiom~\eqref{def:orig:inner:and-break-right},
      $\delta=\<\clear(p'),\alpha,m>$, and by~\Cref{def:orig:blocked},
      \begin{align*}
        \blocked(\ceu{p'\And\;\Break})
        &=\blocked(p')\cdot\blocked(\ceu{\Break},\alpha,n)\\
        &=1\cdot0=0.
      \end{align*}

    \item\label{thm:orig:lemma:and}
      $p',p''\ne\ceu{\Skip},\ceu{\Break}$.  By induction
      hypothesis, exactly one of the following hold:
      \[
        \exists{d'\in\Delta}(\<p',\alpha,m>\step{n}d')
        \quad\text{or}\quad
        \blocked(p',\alpha,n)=1.
      \]

      If~$\<p',\alpha,m>\step{n}\<p_1',\alpha',m'>$, for some~$p_1'\in{P}$,
      $\alpha'\in{E^*}$, and~$m'\in\mathcal{M}$, then by
      rule~\eqref{def:orig:inner:and-left},
      \[
        \<\ceu{p'\And{p''}},\alpha,m>
        \step{n}\<\ceu{p'_1\And{p''}},\alpha',m'>.
      \]
      And by \Cref{def:orig:blocked},
      \begin{align*}
        \blocked(\ceu{p'\And{p''}},\alpha,n)
        &=\blocked(p',\alpha,n)\cdot\blocked(p'',\alpha,n)\\
        &=0\cdot\blocked(p'',\alpha,n)=0.
      \end{align*}

      If, however,~$\blocked(p',\alpha,n)=1$ then, again, by induction
      hypothesis,
      \[
        \exists{d''\in\Delta}(\<p'',\alpha,m>\step{n}d'')
        \quad\text{or}\quad
        \blocked(p'',\alpha,n)=1,
      \]
      but not both.  Suppose~$\<p'',\alpha,m>\step{n}\<p_2'',\alpha',m'>$,
      for some~$p_2''\in{P}$, $\alpha'\in{E^*}$, and~$m'\in\mathcal{M}$.
      Then by rule~\eqref{def:orig:inner:and-right},
      \[
        \<\ceu{p'\And{p''}},\alpha,m>
        \step{n}\<\ceu{p'\And{p_2''}},\alpha',m'>,
      \]
      and by \Cref{def:orig:blocked},
      \begin{align*}
        \blocked(\ceu{p'\And{p''}},\alpha,n)
        &=\blocked(p',\alpha,n)\cdot\blocked(p'',\alpha,n)\\
        &=1\cdot0=0.
      \end{align*}
      Suppose~$\blocked(p'',\alpha,n)=1$.  Then there is no such~$\delta$
      (no rule is applicable) and by \Cref{def:orig:blocked},
      \begin{align*}
        \blocked(\ceu{p'\And{p''}},\alpha,n)
        &=\blocked(p',\alpha,n)\cdot\blocked(p'',\alpha,n)\\
        &=1\cdot1=1.
      \end{align*}
    \end{case}
    %%
  \item$p=\ceu{p'\Or{p''}}$.
    \begin{case}
    \item$p'=\ceu{\Skip}$.  By axiom~\eqref{def:orig:inner:or-skip-left},
      $\delta=\<\ceu{\clear(p'')},\alpha,m>$, and
      by~\Cref{def:orig:blocked},
      \begin{align*}
        \blocked(\ceu{\Skip\Or\;p''},\alpha,n)
        &=\blocked(\ceu{\Skip},\alpha,n)
          \cdot\blocked(p'',\alpha,n)\\
        &=0.
      \end{align*}
    \item $p'\ne\ceu{\Skip,\Break}$ and~$p''=\ceu{\Skip}$.  By
      induction hypothesis, exactly one of the following hold:
      \[
        \exists{d'\in\Delta}(\<p',\alpha,m>\step{n}d')
        \quad\text{or}\quad
        \blocked(p',\alpha,n)=1.
      \]

      If~$\blocked(p',\alpha,n)=0$, this case
      becomes~\Cref{thm:orig:lemma:or}.

      If, however,~$\blocked(p',\alpha,n)=1$, then by
      axiom~\eqref{def:orig:inner:or-skip-right},
      $\delta=\<\ceu{\clear(p')},\alpha,m>$, and by \Cref{def:orig:blocked},
      \begin{align*}
        \blocked(\ceu{p'\Or\;\Skip},\alpha,n)
        &=\blocked(p',\alpha,n)\cdot\blocked(\ceu\Skip,\alpha,n)\\
        &=1\cdot0=0.
      \end{align*}
    \item$p'=\ceu{\Break}$.  By axiom~\eqref{def:orig:inner:or-break-left},
      $\delta=\<\ceu{\clear(p'');\Break},\alpha,m>$, and
      by~\Cref{def:orig:blocked},
      \begin{align*}
        \blocked(\ceu{\Break\Or\;p''})
        &=\blocked(\ceu{\Break})\cdot\blocked(p'',\alpha,n)\\
        &=0.
      \end{align*}
    \item $p'\ne\ceu{\Skip,\Break}$ and~$p''=\ceu\Break$.  By
      induction hypothesis, exactly one of the following hold:
      \[
        \exists{d'\in\Delta}(\<p',\alpha,m>\step{n}d')
        \quad\text{or}\quad
        \blocked(p',\alpha,n)=1.
      \]

      If~$\blocked(p',\alpha,n)=0$, this case becomes
      \Cref{thm:orig:lemma:or}.

      If, however,~$\blocked(p',\alpha,n)=1$, then by
      axiom~\eqref{def:orig:inner:or-break-right},
      $\delta=\<\ceu{\clear(p');\Break},\alpha,m>$, and
      by~\Cref{def:orig:blocked},
      \begin{align*}
        \blocked(\ceu{p'\Or\;\Break})
        &=\blocked(p')\cdot\blocked(\ceu{\Break},\alpha,n)\\
        &=1\cdot0=0.
      \end{align*}
    \item\label{thm:orig:lemma:or}
      $p',p''\ne\ceu{\Skip},\ceu{\Break}$.  By induction
      hypothesis, exactly one of the following hold:
      \[
        \exists{d'\in\Delta}(\<p',\alpha,m>\step{n}d')
        \quad\text{or}\quad
        \blocked(p',\alpha,n)=1.
      \]

      If~$\<p',\alpha,m>\step{n}\<p_1',\alpha',m'>$, for some~$p_1'\in{P}$,
      $\alpha'\in{E^*}$, and~$m'\in\mathcal{M}$, then by
      rule~\eqref{def:orig:inner:or-left},
      \[
        \<\ceu{p'\Or{p''}},\alpha,m>
        \step{n}\<\ceu{p'_1\Or{p''}},\alpha',m'>.
      \]
      And by \Cref{def:orig:blocked},
      \begin{align*}
        \blocked(\ceu{p'\Or{p''}},\alpha,n)
        &=\blocked(p',\alpha,n)\cdot\blocked(p'',\alpha,n)\\
        &=0\cdot\blocked(p'',\alpha,n)=0.
      \end{align*}

      If, however,~$\blocked(p',\alpha,n)=1$ then, again, by induction
      hypothesis,
      \[
        \exists{d''\in\Delta}(\<p'',\alpha,m>\step{n}d'')
        \quad\text{or}\quad
        \blocked(p'',\alpha,n)=1,
      \]
      but not both.  Suppose~$\<p'',\alpha,m>\step{n}\<p_2'',\alpha',m'>$,
      for some~$p_2''\in{P}$, $\alpha'\in{E^*}$, and~$m'\in\mathcal{M}$.
      Then by rule~\eqref{def:orig:inner:or-right},
      \[
        \<\ceu{p'\Or{p''}},\alpha,m>
        \step{n}\<\ceu{p'\Or{p_2''}},\alpha',m'>,
      \]
      and by \Cref{def:orig:blocked},
      \begin{align*}
        \blocked(\ceu{p'\Or{p''}},\alpha,n)
        &=\blocked(p',\alpha,n)\cdot\blocked(p'',\alpha,n)\\
        &=1\cdot0=0.
      \end{align*}
      Suppose~$\blocked(p'',\alpha,n)=1$.  Then there is no such~$\delta$
      (no rule is applicable) and by \Cref{def:orig:blocked},
      \begin{align*}
        \blocked(\ceu{p'\Or{p''}},\alpha,n)
        &=\blocked(p',\alpha,n)\cdot\blocked(p'',\alpha,n)\\
        &=1\cdot1=1.\qedhere
      \end{align*}
    \end{case}
  \end{case}
\end{proof}
