\begin{proof}
  By induction on the structure of derivations.
  Suppose
  \[
    d_1\Vdash\<p,\alpha,m>\ostep{n}\<p_1,\alpha_1,m_1>
    \quad\text{and}\quad
    d_2\Vdash\<p,\alpha,m>\ostep{n}\<p_2,\alpha_2,m_2>,
  \]
  for some derivations~$d_1$ and~$d_2$.  Then there are twelve possibilities
  depending on the structure of~$p$.  (Note that~$p$ cannot be equal
  to~$\ceu{\Skip}$, $\ceu{\Attr{v}{a}}$, or $\ceu{\Break}$, as there are no
  rules to evaluate such programs.)

  \begin{case}  
  \item$p=\ceu{\Await(e)}$, for some~$e\in{E}$.  By \Cref{def:orig:blocked}
    $\blocked(\ceu{\Await(e)},\alpha,m) = 0$, therefre $d_1$ and~$d_2$ are
    instances of rule~\eqref{def:orig:outer:advance} and as such,
    $p_1=p_2=\ceu{\Awaiting(e,n')}$ with~$n'=n+1$, and
    $\alpha_1=\alpha_2=\alpha$ and~$m_1=m_2=m$.
    %%
  \item$p=\ceu{\Awaiting(e,n')}$, for some~$e\in{E}$ and~$n'\in{N}$.
    \begin{case}
      \item
    \end{case}

    By \Cref{def:orig:blocked}
    $\blocked(\ceu{\Await(e)},\alpha,m) = 0$, therefre $d_1$ and~$d_2$ are
    instances of rule~\eqref{def:orig:outer:advance} and as such,
    $p_1=p_2=\ceu{\Skip}$, $\alpha_1=\alpha_2=\alpha$, and~$m_1=m_2=m$.
    %%
  \item$p=\ceu{\Emit(e)}$, for some~$e\in{E}$.  Then~$d_1$ and~$d_2$ are
    instances of axiom~\eqref{def:orig:inner:emit}, and as such,
    $p_1=p2=\ceu{\Emitting(n')}$ with~$n'=\|\alpha|$,
    and~$\alpha_1=\alpha_2=e\alpha$ and~$m_1=m_2=m$.
    %%
  \item$p=\ceu{\Emitting(e,n')}$, for some~$e\in{E}$ and~$n'\in{N}$.
    Then~$d_1$ and~$d_2$ are instances of
    axiom~\eqref{def:orig:inner:emitting} with~$n'=\|\alpha|$.
    Thus~$p_1=p_2=\ceu{\Skip}$, $\alpha_1=\alpha_2=\alpha$ and~$m_1=m_2=m$.
    %%
  \item$p=\ceu{\Ifelse{b}{p'}{p''}}$, for some~$b\in{B}$ and~$p'$,
    $p''\in{P}$.
    \begin{case}
    \item$\eval(b,m)=1$.  Then~$d_1$ and~$d_2$ are instances of
      axiom~\eqref{def:orig:inner:if-true}, and as such, $p_1=p_2=p'$,
      $\alpha_1=\alpha_2=\alpha$, and~$m_1=m_2=m$.
    \item$\eval(b,m)=0$.  Then~$d_1$ and~$d_2$ are instances of
      axiom~\eqref{def:orig:inner:if-false}, and as such, $p_1=p_2=p''$,
      $\alpha_1=\alpha_2=\alpha$, and~$m_1=m_2=m$.
    \end{case}
  \item$p=\ceu{p';p''}$, for some~$p'$, $p''\in{P}$.
    \begin{case}
    \item$p'=\ceu\Skip$.  Then~$d_1$ and~$d_2$ are instances of
      axiom~\eqref{def:orig:inner:seq-skip}, and as such, $p_1=p_2=p''$,
      $\alpha_1=\alpha_2=\alpha$ and $m_1=m_2=m$.
    \item$p'=\ceu{\Attr{v}{a}}$, for some~$v\in{V}$ and~$a\in{A}$.
      Then~$d_1$ and~$d_2$ are instances of
      axiom~\eqref{def:orig:inner:seq-attr}, and as such, $p_1=p_2=p''$,
      $\alpha_1=\alpha_2=\alpha$ and, as~$\eval$ is a total function,
      $m_1=m_2=m[v/\eval(a)]$.
    \item$p'=\ceu{\Break}$.  Then~$d_1$ and~$d_2$ are instances of
      axiom~\eqref{def:orig:inner:seq-break}, and as such, $p_1=p_2=p'$,
      $\alpha_1=\alpha_2=\alpha$ and~$m_1=m_2=m$.
    \item$p'\ne\ceu{\Skip,\Attr{v}{a}},\ceu{\Break}$.  Then~$d_1$ and~$d_2$
      are instances of rule~\eqref{def:orig:inner:seq}.  Thus there are
      derivations~$d_1'$ and~$d_2'$ such that
      \begin{align*}
        d_1'\Vdash\<p',\alpha,m>\step{n}\<p_1',\alpha_1,m_1>
        \quad\text{and}\quad
        d_2'\Vdash\<p',\alpha,m>\step{n}\<p_2',\alpha_2,m_2>,
      \end{align*}
      for some~$p_1'$, $p_2'\in{P}$.  Since~$d_1'\prec{d_1}$
      and~$d_2'\prec{d_2}$, by induction hypothesis, $\alpha_1=\alpha_2$,
      $m_1=m_2$, and~$p_1'=p_2'$, which implies
      \[
        p_1=p_1';p''=p_2';p''=p_2.
      \]
    \end{case}
    %%
  \item$p=\ceu{\Loop{p'}}$, for some~$p'\in{P}$.  Then~$d_1$ and~$d_2$ are
    instances of axiom~\eqref{def:orig:inner:loop}, and as such,
    $p_1=p_2=\ceu{p'\Atloop{p'}}$, $\alpha_1=\alpha_2=\alpha$,
    and~$m_1=m_2=m$.
    %%
  \item$p=\ceu{p'\Atloop{p''}}$, for some~$p'$, $p''\in{P}$.
    \begin{case}
    \item$p=\ceu{\Skip\Atloop{p'}}$, for some~$p'\in{P}$.  Then~$d_1$
      and~$d_2$ are instances of axiom~\eqref{def:orig:inner:atloop-skip},
      and as such, $p_1=p_2=\ceu{\Loop{p'}}$, $\alpha_1=\alpha_2=\alpha$,
      and~$m_1=m_2=m$.
    \item$p=\ceu{\Attr{v}{a}\Atloop{p'}}$, for some~$a\in{A}$, $v\in{V}$,
      and~$p'\in{P}$.  Then~$d_1$ and~$d_2$ are instances
      of axiom~\eqref{def:orig:inner:atloop-attr}, and as such,
      $p_1=p_2=\ceu{\Loop{p'}}$, $\alpha_1=\alpha_2=\alpha$, and as~$\eval$
      is a total function, $m_1=m_2=m[v/\eval(a)]$.
    \item$p=\ceu{\Break\Atloop{p'}}$, for some~$p'\in{P}$.  Then~$d_1$
      and~$d_2$ are instances of axiom~\eqref{def:orig:inner:atloop-break},
      and as such, $p_1=p_2=\ceu{\Skip}$, $\alpha_1=\alpha_2=\alpha$,
      and~$m_1=m_2=m$.
    \item$p=\ceu{p'\Atloop{p''}}$, for some~$p'$, $p''\in{P}$ such
      that~$p'\ne\ceu{\Skip,\Attr{v}{a}},\ceu{\Break}$.  Then~$d_1$
      and~$d_2$ are instances of rule~\eqref{def:orig:inner:atloop}.  Thus
      there are derivations~$d_1'$ and~$d_2'$ such that
      \[
        d_1'\Vdash\<p',\alpha,m>\step{n}\<p_1',\alpha_1,m_1>
        \quad\text{and}\quad
        d_2'\Vdash\<p',\alpha,m>\step{n}\<p_2',\alpha_2,m_2>,
      \]
      for some~$p_1'$, $p_2'\in{P}$.  Since~$d_1'\prec{d_1}$
      and~$d_2'\prec{d_2}$, by induction hypothesis, $\alpha_1=\alpha$,
      $m_1=m_2$, and~$p_1'=p_2'$, which implies
      \[
        p_1=\ceu{p_1'\Atloop{p''}}=\ceu{p_2'\Atloop{p''}}=p_2.
      \]
    \end{case}
    %%
  \item\label{thm:orig:det-inner:and} $p=\ceu{p'\And{p''}}$, for some~$p'$,
    $p''\in{P}$.
    \begin{case}
    \item\label{thm:orig:det-inner:and-skip-left}
      $p=\ceu{\Skip\And{\;p'}}$, for some~$p'\in{P}$
      \MARK{and $p'\ne \ceu\Break$}.
      Then~$d_1$ and~$d_2$ are instances of
      axiom~\eqref{def:orig:inner:and-skip-left}, and as such, $p_1=p_2=p'$,
      $\alpha_1=\alpha_2=\alpha$, and $m_1=m_2=m$.
    \item$p=\ceu{p'\And\Skip}$, for some~~$p'\in{P}$ 
      \MARK{and $p'\ne \ceu\Break$}.
      Similar to \Cref{thm:orig:det-inner:and-skip-left}.
    \item\label{thm:orig:det-inner:and-attr-left}
      $p=\ceu{\Attr{v}{a}\And{p'}}$, for some~$v\in{V}$, $a\in{A}$
      and~$p'\in{P}$.  Then~$d_1$ and~$d_2$ are instances of
      axiom~\eqref{def:orig:inner:and-attr-left}, and as such, $p_1=p_2=p'$,
      $\alpha_1=\alpha_2=\alpha$, and as~$\eval$ is a total function,
      $m_1=m_2=m[v/\eval(a)]$.
    \item$p=\ceu{p'\And\Attr{v}{a}}$, for some~$v\in{V}$, $a\in{A}$
      and~$p'\in{P}$.  Then either~$\blocked(p')=0$ or~$\blocked(p')=1$.
      If~$\blocked(p')=0$ then this case becomes
      \Cref{thm:orig:det-inner:and-left}.  Otherwise, if~$\blocked(p')=1$,
      then~$d_1$ and~$d_2$ are instances of
      axiom~\eqref{def:orig:inner:and-attr-right}, and as such,
      $p_1=p_2=p'$, $\alpha_1=\alpha_2=\alpha$, and as~$\eval$ is a total
      function, $m_1=m_2=m[v/\eval(a)]$.
    \item$p=\ceu{\Break\And{\;p'}}$, for some~$p'\in{P}$.  Then~$d_1$
      and~$d_2$ are instances of
      axiom~\eqref{def:orig:inner:and-break-left}, and as such,
      $\alpha_1=\alpha_2=\alpha$, $m_1=m_2=m$, and as~$\clear$ is a total
      function, $p_1=p_2=\ceu{\clear(p');\Break}$.
    \item$p=\ceu{{p'}\And\Break}$, for some~$p'\in{P}$.  Then
      either~$\blocked(p')=0$ or~$\blocked(p')=1$.  If~$\blocked(p')=0$ then
      this case becomes \Cref{thm:orig:det-inner:and-left}.  Otherwise,
      if~$\blocked(p')=1$, then~$d_1$ and~$d_2$ are instances of
      axiom~\eqref{def:orig:inner:and-break-right}, and as such,
      $\alpha_1=\alpha_2=\alpha$, $m_1=m_2=m$, and as~$\clear$ is a total
      function, $p_1=p_2=\ceu{\clear(p');\Break}$.
    \item\label{thm:orig:det-inner:and-left} $p=\ceu{p'\And{p''}}$, for
      some~$p'$ and~$p''\in{P}$.  Then there are two possibilities.
      If~$\blocked(p')=0$ then~$d_1$ and~$d_2$ are instances
      of~\eqref{def:orig:inner:and-left}.  Thus there are derivations~$d_1'$
      and~$d_2'$ such that
      \[
        d_1'\Vdash\<p',\alpha,m>\step{n}\<p_1',\alpha_1,m_1>
        \quad\text{and}\quad
        d_2'\Vdash\<p',\alpha,m>\step{n}\<p_2',\alpha_2,m_2>,
      \]
      for some~$p_1'$, $p_2'\in{P}$.  Since~$d_1'\prec{d_1}$
      and~$d_2'\prec{d_2}$, by induction hypothesis, $\alpha_1=\alpha_2$,
      $m_1=m_2$, and~$p_1'=p_2'$, which implies
      \[
        p_1=(\ceu{p_1'\And{p''}})=(\ceu{p_2'\And{p''}})=p_2.
      \]

      If, however, $\blocked(p')=1$ and
      $p''\ne\ceu{\Skip,\Attr{v}{a},\Break}$, then~$d_1$ and~$d_2$ are
      instances of~~\eqref{def:orig:inner:and-right}.  Thus there are
      derivations~$d_1''$ and~$d_2''$ such that
      \[
        d_1''\Vdash\<p'',\alpha,m>\step{n}\<p_1'',\alpha_1,m_1>
        \quad\text{and}\quad
        d_2''\Vdash\<p'',\alpha,m>\step{n}\<p_2'',\alpha_2,m_2>,
      \]
      for some~$p_1''$, $p_2''\in{P}$.  Since~$d_1''\prec{d_1}$
      and~$d_2''\prec{d_2}$, by induction hypothesis, $\alpha_1=\alpha_2$,
      $m_1=m_2$, and~$p_1''=p_2''$, which implies
      \[
        p_1=(\ceu{p'\And{p_1''}})=(\ceu{p'\And{p_2''}})=p_2.
      \]
    \end{case}
    %%
  \item$p=\ceu{p'\Or{p''}}$, for some~$p'$, $p''\in{P}$.
    \begin{case}
    \item$p=\ceu{\Skip\Or{\;p'}}$, for some~$p'\in{P}$.  Then~$d_1$
      and~$d_2$ are instances of axiom~\eqref{def:orig:inner:or-skip-left},
      and as such, $\alpha_1=\alpha_2=\alpha$, $m_1=m_2=m$, and as~$\clear$
      is a total, $p_1=p_2=\ceu\clear(p')$.
    \item$p=\ceu{p'\Or\Skip}$, for some~$p'\in{P}$.  Then
      either~$\blocked(p')=0$ or~$\blocked(p')=1$.  If~$\blocked(p')=0$ then
      this case becomes \Cref{thm:orig:det-inner:or-left}.  Otherwise,
      if~$\blocked(p')=1$, then~$d_1$ and~$d_2$ are instances of
      axiom~\eqref{def:orig:inner:or-skip-right}, and as such,
      $\alpha_1=\alpha_2=\alpha$, $m_1=m_2=m$, and as~$\clear$ is a total
      function, $p_1=p_2=\ceu\clear(p')$.
    \item\label{thm:orig:det-inner:or-attr-left}
      $p=\ceu{\Attr{v}{a}\Or{p'}}$, for some~$v\in{V}$, $a\in{A}$
      and~$p'\in{P}$.  Then~$d_1$ and~$d_2$ are instances of
      axiom~\eqref{def:orig:inner:or-attr-left}, and as such,
      $\alpha_1=\alpha_2=\alpha$, and as~$\eval$ and~$\clear$ are total
      functions, $m_1=m_2=m[v/\eval(a)]$ and~$p_1=p_2=\ceu\clear(p')$.
    \item$p=\ceu{p'\Or\Attr{v}{a}}$, for some~$v\in{V}$, $a\in{A}$
      and~$p'\in{P}$.  Then either~$\blocked(p')=0$ or~$\blocked(p')=1$.
      If~$\blocked(p')=0$ then this case becomes
      \Cref{thm:orig:det-inner:or-left}.  Otherwise, if~$\blocked(p')=1$,
      then~$d_1$ and~$d_2$ are instances of
      axiom~\eqref{def:orig:inner:or-attr-right}, and as such,
      $\alpha_1=\alpha_2=\alpha$, and as~$\eval$ and~$\clear$ are total
      functions, $m_1=m_2=m[v/\eval(a)]$ and~$p_1=p_2=\ceu\clear(p')$.
    \item$p=\ceu{\Break\Or{\;p'}}$, for some~$p'\in{P}$.  Then~$d_1$
      and~$d_2$ are instances of axiom~\eqref{def:orig:inner:or-break-left},
      and as such, $\alpha_1=\alpha_2=\alpha$, $m_1=m_2=m$, and as~$\clear$
      is a total function, $p_1=p_2=\ceu{\clear(p');\Break}$.
    \item$p=\ceu{{p'}\Or\Break}$, for some~$p'\in{P}$.  Then
      either~$\blocked(p')=0$ or~$\blocked(p')=1$.  If~$\blocked(p')=0$ then
      this case becomes \Cref{thm:orig:det-inner:or-left}.  Otherwise,
      if~$\blocked(p')=1$, then~$d_1$ and~$d_2$ are instances of
      axiom~\eqref{def:orig:inner:or-break-right}, and as such,
      $\alpha_1=\alpha_2=\alpha$, $m_1=m_2=m$, and as~$\clear$ is a total
      function, $p_1=p_2=\ceu{\clear(p');\Break}$.
    \item\label{thm:orig:det-inner:or-left}$p=\ceu{p'\Or{p''}}$, for
      some~$p'$ and~$p''\in{P}$.  Then there are two possibilities.
      If~$\blocked(p')=0$ then~$d_1$ and~$d_2$ are instances
      of~\eqref{def:orig:inner:or-left}.  Thus there are derivations~$d_1'$
      and~$d_2'$ such that
      \[
        d_1'\Vdash\<p',\alpha,m>\step{n}\<p_1',\alpha_1,m_1>
        \quad\text{and}\quad
        d_2'\Vdash\<p',\alpha,m>\step{n}\<p_2',\alpha_2,m_2>,
      \]
      for some~$p_1'$, $p_2'\in{P}$.  Since~$d_1'\prec{d_1}$
      and~$d_2'\prec{d_2}$, by induction hypothesis, $\alpha_1=\alpha_2$,
      $m_1=m_2$, and~$p_1'=p_2'$, which implies
      \[
        p_1=(\ceu{p_1'\Or{p''}})=(\ceu{p_2'\Or{p''}})=p_2.
      \]
      If, however, $\blocked(p')=1$ and
      $p''\ne\ceu{\Skip,\Attr{v}{a},\Break}$, then~$d_1$ and~$d_2$ are
      instances of~~\eqref{def:orig:inner:or-right}.  Thus there are
      derivations~$d_1''$ and~$d_2''$ such that
      \[
        d_1''\Vdash\<p'',\alpha,m>\step{n}\<p_1'',\alpha_1,m_1>
        \quad\text{and}\quad
        d_2''\Vdash\<p'',\alpha,m>\step{n}\<p_2'',\alpha_2,m_2>,
      \]
      for some~$p_1''$, $p_2''\in{P}$.  Since~$d_1''\prec{d_1}$
      and~$d_2''\prec{d_2}$, by induction hypothesis, $\alpha_1=\alpha_2$,
      $m_1=m_2$, and~$p_1''=p_2''$, which implies
      \[
        p_1=(\ceu{p'\Or{p_1''}})=(\ceu{p'\Or{p_2''}})=p_2.\qedhere
      \]
    \end{case}
  \end{case}
\end{proof}


